\section{Chapter8: Introdcution to Statistics}

\begin{formula}{NOTATION}
    \begin{align*}
        \mu &= \textnormal{population mean}\\
        \bar{X} &= \textnormal{Sample mean, estimator of $\mu$}\\
        &\\
        \sigma &= \textnormal{population standard deviation}\\
        s &= \textnormal{sample standard deviation, estimator of $\sigma$}\\
        &\\
        \sigma^2 &= \textnormal{population variance}\\
        s^2 &= \textnormal{sample variance, estimator of $\sigma$} \\
        &\\
        \sigma(\hat{\theta}) &= \textnormal{standard error of estimator $\hat{\theta}$ of parameter $\theta$}\\
        s(\hat{\theta}) &= \textnormal{estimated standard error = $\hat{\sigma}(\hat{\theta})$}
    \end{align*}
\end{formula}

\subsection{Mean}

\paragraph{\textit{Population Mean:}} $\mu = \expc{X}$

\paragraph{\textit{Sample Mean}}
\begin{equation*}
    \bar{X} = \frac{X_1 + \cdots + X_n}{n}
\end{equation*}

\subsubsection{Unbiasedness}

\paragraph{Unbiased}
\begin{equation*}
    \expc{\hat{\theta}} = \theta
\end{equation*}

Bias of $\hat{\theta}$ is defined as Bias($\hat{\theta}$) = $\expc{\hat{\theta} - \theta}$.

\subsection{Variance and Standard Deviation}

\paragraph{Sample Variance}
\begin{equation*}
    s^2 = \frac{1}{n - 1} \sum_{i = 1}^{n} (X_i - \bar{X})^2
\end{equation*}
Another formula
\begin{equation*}
    s^2 = \frac{\dsum_{i=1}^n X_i^2 - n\bar{X}^2}{n-1}
\end{equation*}

\paragraph{Sample Standard Deviation}
\begin{equation*}
    s = \sqrt{s^2}
\end{equation*}

\paragraph{Variance of $\bar{X}$}
\begin{equation*}
    \var{\bar{X}} = \frac{\sigma^2}{n}
\end{equation*}

\paragraph{Standard Deviation of $\bar{X}$}
\begin{equation*}
    \sigma(\bar{X}) = \sqrt{\var{\bar{X}}} = \sqrt{\frac{\sigma^2}{n}} = \frac{\sigma}{\sqrt{n}}
\end{equation*}

\subsection{Standard Errors of Estimates}

\textbf{Standard error} of an estimator $\hat{\theta}$ is its standard deviation, $\sigma(\hat{\theta}) = \textnormal{Std}(\hat{\theta})$
